Hashtable: Rewrote several basic definitions. Begin work on insert_spec.

iterators/hashtable.v
@@ -14,21 +14,21 @@ Section HashTable.
   Variable array : val -> list val -> iProp Σ.
 
   Hypothesis modulo_spec:
-    forall (m n : Z),  WP modulo #m #n {{v, ⌜v = #(m `mod` n)⌝}}%I.
+    forall (m n : Z), WP modulo (#m, #n) {{v, ⌜v = #(m `mod` n)⌝}}%I.
 
   Hypothesis make_array_spec:
-    forall (n : nat) (v : val), WP make_array #n v {{arr, array arr (replicate n v)}}%I.
+    forall (n : nat) (v : val), WP make_array (#n, v) {{arr, array arr (replicate n v)}}%I.
 
   Hypothesis array_load_spec:
     forall arr xs v (n : nat),
-      xs !! n = Some v -> {{array arr xs}} array_load arr #n {{u, ⌜u = v⌝ ∗ array arr xs}}%I.
+      xs !! n = Some v -> {{array arr xs}} array_load (arr, #n) {{u, ⌜u = v⌝ ∗ array arr xs}}%I.
 
   Hypothesis array_store_spec:
     forall arr xs (v : val) (n : nat),
-      length xs < n -> {{array arr xs}} array_store arr #n v {{_, array arr (<[n := v]> xs)}}%I.
+      n < length xs -> {{array arr xs}} array_store (arr, #n, v) {{_, array arr (<[n := v]> xs)}}%I.
 
-  Notation "e1 .[ e2 ]" := (array_load e1%E e2%E) (at level 20): expr_scope.
-  Notation "e1 .[ e2 ] := e3" := (array_store e1%E e2%E e3%E) (at level 20): expr_scope.
+  Notation "e1 .[ e2 ]" := (array_load (e1, e2)%E) (at level 20): expr_scope.
+  Notation "e1 .[ e2 ] := e3" := (array_store (e1, e2, e3)%E) (at level 20): expr_scope.
 
   Structure Hashable := mkHashable {
     equal : val;
@@ -38,22 +38,21 @@ Section HashTable.
     key_eq : EqDecision Key;
     key_countable : Countable Key;
     Hash : Key -> nat;
-    compat : Proper (eq ==> eq) Hash;
-    is_key : Key -> val -> Prop;
-    is_key_decision : forall k v, Decision (is_key k v);
+    as_key : val -> option Key;
     
-    equal_spec_true (k1 k2: Key) (v1 v2: val) :
-      (k1 = k2) -> is_key k1 v1 -> is_key k2 v2 ->
+    equal_spec_true (k: Key) (v1 v2: val) :
+      as_key v1 = Some k ->
+      as_key v2 = Some k ->
       WP equal v1 v2 {{u, ⌜u = #true⌝}}%I;
 
     equal_spec_false k1 k2 v1 v2 :
-      (k1 ≠ k2) -> is_key k1 v1 -> is_key k2 v2 ->
+      (k1 ≠ k2) -> as_key v1 = Some k1 -> as_key v2 = Some k2 ->
       WP equal v1 v2 {{u, ⌜u = #false⌝}}%I;
 
-    hash_spec k v : is_key k v -> WP hash v {{u, ⌜u = #(Hash k)⌝}}%I;
+    hash_spec k v : as_key v = Some k -> WP hash v {{u, ⌜u = #(Hash k)⌝}}%I;
   }.
 
-  Existing Instances key_eq key_countable compat is_key_decision.
+  Existing Instances key_eq key_countable.
 
   Structure HashTable (K : Hashable) := hashTable {
     create : val;
@@ -68,30 +67,57 @@ Section HashTable.
     
 
     Definition create_impl : val :=
-      λ: "n" , (ref (make_array "n" NONE), ref #0, ref "n").
+      λ: "n" , (ref (make_array ("n", NONE)), ref #0, ref "n").
 
     Definition index : val :=
-      λ: "t" "k", modulo (hash K "k") !(Snd (Snd "t")).
+      λ: "t" "k", modulo (hash K "k", !(Snd "t")).
 
-    Definition resize : val :=
-      λ: "t", let: "old" := !(Fst "t") in
-              let: "size" :=  !(Snd (Snd "t")) in
-              Fst "t" <- make_array ("size" + "size") NONE;;
-              Snd (Snd "t") <- "size" + "size";;
-              let: "loop" :=
-                 rec: "loop" "i" :=
-                   if: "i" < "size" then
+    Definition resize_loop : val :=
+      rec: "loop" "cap" "old" "t" "i" :=
+                   if: "i" < "cap" then
                      let: "mv_buck" :=
                         rec: "mv_buck" "b" :=
                           match: "b" with
                             NONE => #()
                           | SOME "a"
-                            => let: "k" := Fst "a" in
-                               let: "x" := Fst (Snd "a") in
-                               let: "b'" := Snd (Snd "a") in
+                            => let: "k" := Fst (Fst "a") in
+                               let: "x" := Snd (Fst "a") in
+                               let: "b'" := Snd "a" in
                                "mv_buck" "b'";;
                                let: "idx" := index "t" "k" in
-                               (!(Fst "t")).["idx"] := SOME ("k", "x", (!(Fst "t")).["idx"])
+                               (!(Fst (Fst "t"))).["idx"] := SOME ("k", "x", (!(Fst (Fst "t"))).["idx"])
+                          end
+                     in
+                     "mv_buck" ("old".["i"]);;
+                     "loop" ("i" + #1)
+                   else #().
+
+    Definition resize : val :=
+      λ: "t", let: "old" := !(Fst (Fst "t")) in
+              let: "cap" :=  !(Snd "t") in
+              Fst (Fst "t") <- make_array ("cap" + "cap", NONE);;
+              Snd "t" <- "cap" + "cap";;
+              resize_loop "cap" "old" "t" #0.
+    
+    Definition resize2 : val :=
+      λ: "t", let: "old" := !(Fst (Fst "t")) in
+              let: "cap" :=  !(Snd "t") in
+              Fst (Fst "t") <- make_array ("cap" + "cap", NONE);;
+              Snd "t" <- "cap" + "cap";;
+              let: "loop" :=
+                 rec: "loop" "i" :=
+                   if: "i" < "cap" then
+                     let: "mv_buck" :=
+                        rec: "mv_buck" "b" :=
+                          match: "b" with
+                            NONE => #()
+                          | SOME "a"
+                            => let: "k" := Fst (Fst "a") in
+                               let: "x" := Snd (Fst "a") in
+                               let: "b'" := Snd "a" in
+                               "mv_buck" "b'";;
+                               let: "idx" := index "t" "k" in
+                               (!(Fst (Fst "t"))).["idx"] := SOME ("k", "x", (!(Fst (Fst "t"))).["idx"])
                           end
                      in
                      "mv_buck" ("old".["i"]);;
@@ -101,12 +127,12 @@ Section HashTable.
                       
     Definition insert_impl : val :=
       λ: "t" "k" "x", let: "i" := index "t" "k" in
-                      (!(Fst "t")).["i"] := SOME ("k", "x", (!(Fst "t")).["i"]);;
-                      let: "size" := #1 + !(Fst(Snd "t")) in
+                      (!(Fst (Fst "t"))).["i"] := SOME ("k", "x", (!(Fst (Fst "t"))).["i"]);;
+                      let: "size" := #1 + !(Snd(Fst "t")) in
                       Snd(Fst "t") <- "size" ;;
-                      let: "cap" := !(Snd (Snd "t")) in
-                      if:  "cap" + "cap" < "size" then
-                        resize "t" else #().
+                      let: "cap" := !(Snd "t") in
+                      (*if:  "cap" + "cap" < "size" then
+                        resize "t" else *) #().
                                                  
     Definition lookup_impl : val :=
       λ: "t" "k", let: "i" := index "t" "k" in
@@ -115,9 +141,9 @@ Section HashTable.
                        match: "b" with
                          NONE => NONE
                        | SOME "a"
-                         => let: "k'" := Fst "a" in
-                            let: "x" := Fst (Snd "a") in
-                            let: "b'" := Snd (Snd "a") in
+                         => let: "k'" := Fst (Fst "a") in
+                            let: "x" := Snd (Fst "a") in
+                            let: "b'" := Snd "a" in
                             if: (equal K) "k" "k'" then
                               SOME "x"
                             else
@@ -125,43 +151,148 @@ Section HashTable.
                        end
                   in "lookup_buck" (!(Fst "t")).["i"].
 
-    Implicit Type M : gmap (Key K) (list val).
+    Implicit Type M : Key K -> list val.
+
+    Instance insertM: Insert (Key K) (val) (Key K -> list val) :=
+      fun k x M k' => if decide (k = k')
+                      then x :: M k'
+                      else M k'.
+
+    
 
     Definition BucketData := list (val * val).
-    
 
     Fixpoint bucket (kvs : BucketData) : val :=
       match kvs with
       | [] => NONEV
       | (k, x) :: tl => SOMEV (k, x, bucket tl)
       end.
-    
+
+    Definition lookupData `(data : list (list A)) k :=
+      from_option id []
+                  (data !! (Hash K k mod length data)).
+
+    Definition insertData `(data : list (list A)) k x :=
+      <[(Hash K k mod length data) := x :: lookupData data k ]> data.
+
+    Lemma lookup_mod `(data : list (list A)) k k' :
+      Hash K k mod length data = Hash K k' mod length data ->
+      lookupData data k = lookupData data k'.
+    Proof.
+      intros Hmod.
+      unfold lookupData.
+      rewrite Hmod.
+      f_equal.
+    Qed.
+      
+    Lemma lookup_insert_data `(data : list (list A)) k k' x :
+      0 < length data ->
+      Hash K k mod length data = Hash K k' mod length data ->
+      lookupData (insertData data k' x) k = x :: lookupData data k.
+    Proof.
+      intros Hlen Hmod.
+      unfold insertData.
+      rewrite (lookup_mod _ _ _ Hmod).
+      rewrite -Hmod.
+      unfold lookupData at 1.
+      rewrite insert_length.
+      rewrite Hmod.
+      rewrite list_lookup_insert ; [done|].
+      apply mod_bound_pos.
+      apply le_0_n.
+      done.
+    Qed.
+
+    Lemma lookup_insert_data_other `(data : list (list A)) k k' x :
+      0 < length data ->
+      Hash K k mod length data ≠ Hash K k' mod length data ->
+      lookupData (insertData data k' x) k = lookupData data k.
+    Proof.
+      intros Hlen Hmod.
+      unfold insertData.
+      unfold lookupData at 1.
+      rewrite insert_length.
+      rewrite list_lookup_insert_ne ; [|done].
+      by unfold lookupData.
+    Qed.
+      
     Definition content M (data : list BucketData) :=
       forall k,
-        from_option id [] (M !! k)
-        = map snd (filter (fun p => is_key K k (p.1))
-                          (from_option
-                             id []
-                             (data !! (Hash K k mod length data)))).
+        M k
+        = map snd (filter (fun p => as_key K (p.1) = Some k)
+                          (lookupData data k)).
+
+    Lemma content_insert M data k k' x:
+      0 < length data ->
+      as_key K k' = Some k ->
+      content M data ->
+      content (<[k := x]> M) (insertData data k (k', x)).
+    Proof.
+      intros Hlen HKey HContent k''.
+      unfold base.insert at 1.
+      unfold insertM.
+      destruct (decide (k=k'')) as [<-|].
+      - rewrite lookup_insert_data ; [| done .. ].
+        unfold filter.
+        unfold list_filter.
+        rewrite decide_True ; [| done].
+        simpl.
+        rewrite HContent.
+        done.
+      - destruct (decide (Hash K k mod length data = Hash K k'' mod length data)).
+        + rewrite lookup_insert_data ; [| done ..].
+          unfold filter.
+          unfold list_filter.
+          rewrite decide_False ; [done|].
+          rewrite HKey. by injection.
+        + by rewrite lookup_insert_data_other.
+    Qed.
+    
+      
+    
     
     Definition no_garbage (data : list BucketData) :=
       forall i k,
         i < length data -> 
         i ≠ Hash K k mod length data ->
-        [] = map snd (filter (fun p => is_key K k (p.1))
+        [] = map snd (filter (fun p => as_key K (p.1) = Some k)
                              (from_option
                                 id []
                                 (data !! i))).
 
+    Lemma no_garbage_insert data k k' x :
+      as_key K k' = Some k ->
+      no_garbage data ->
+      no_garbage (insertData data k (k', x)).
+    Proof.
+      intros Hkey HNG i k'' Hlen Hi.
+      unfold insertData in Hi.
+      rewrite insert_length in Hi Hlen.
+      unfold insertData.
+      destruct (decide (i = Hash K k mod length data)).
+      - simplify_eq.
+        rewrite list_lookup_insert ; [|done].
+        simpl. unfold filter. unfold list_filter.
+        simpl.
+        destruct (decide (k = k'')). 
+        simplify_eq.
+        rewrite decide_False.
+        apply HNG ; [|done]. Nat.order.
+        rewrite Hkey.
+        by injection.
+      - rewrite list_lookup_insert_ne ; [|done].
+        apply HNG ; done.
+    Qed.
+      
     Definition TableInState M (lData : loc) (data: list BucketData) (t : val) : iProp Σ:=
       ( ⌜length data > 0⌝ ∗
         ⌜content M data⌝ ∗
         ⌜no_garbage data⌝ ∗
         ∃ (lSize lCap : loc) arr,
           ⌜t = (#lData, #lSize, #lCap)%V⌝ ∗
-          array arr (map bucket data) ∗
+          array arr (fmap bucket data) ∗
           lData ↦ arr ∗
-          lSize ↦ #(map_fold (fun _ l a => a + length l) 0 M) ∗
+          lSize ↦ #(fold_right (fun l a => a + length l) 0 data)%nat ∗
           lCap ↦ #(length data))%I.
 
     Definition Table M (t : val) : iProp Σ :=
@@ -175,13 +306,12 @@ Section HashTable.
       rewrite IHn.
       reflexivity.
     Qed.
-      
-    Print Visibility.
-    Lemma create_impl_spec n : n > 0 -> WP create_impl #n {{t, Table ∅ t}}%I.
+
+    Lemma create_impl_spec n : n > 0 -> WP create_impl #n {{t, Table (const []) t}}%I.
     Proof.
       intro Hn.
       wp_lam.
-      wp_bind (make_array _ _).
+      wp_bind (make_array _).
       iApply (wp_wand).
       iApply (make_array_spec n NONEV ).
       iIntros (arr) "Harr".
@@ -195,12 +325,12 @@ Section HashTable.
       iSplit.
       iPureIntro.
       intro k.
-      rewrite lookup_empty.
+      simpl.
+      unfold lookupData.
       rewrite replicate_length.
-      unfold gt in Hn.
       assert (Hash K k `mod` n < n).
-      { intros. apply Nat.mod_upper_bound. Nat.order. }
-      assert ((replicate n [] !! (Hash K k `mod` n)) = Some ([] : BucketData)) as HSome.     
+      { intros. apply Nat.mod_upper_bound. unfold gt in Hn. Nat.order. }
+      assert ((replicate n [] !! (Hash K k `mod` n)) = Some ([] : BucketData)) as HSome.
       { intros. by rewrite lookup_replicate. }
       by rewrite HSome.
       iSplit.
@@ -214,11 +344,199 @@ Section HashTable.
       iExists lSize, lCap, arr.
       iSplit. done.
       iSplitL "Harr".
-      by rewrite map_replicate.
+      by rewrite fmap_replicate.
       iFrame.
+      iSplitL "HlSize".
+      clear Hn.
+      assert (0 = foldr (λ (l : list (val * val)) (a : nat), a + length l) 0 (replicate n [])) as Hsize.
+      { induction n as [|n IH]. done. simpl. by rewrite -IH. }
+      by rewrite -Hsize.
       by rewrite replicate_length.
+    Qed.
+
+    Lemma index_spec (lArr lSize lCap : loc) (k : val) M k' (data : list val) :
+      as_key K k = Some k' -> {{{lCap ↦ #(length data)}}} index (#lArr, #lSize, #lCap) k {{{RET #(Hash K k' mod length data)%nat ; lCap ↦ #(length data)}}}.
+    Proof.
+      intro HKey.
+      iIntros (Φ) "HlCap HΦ".
+      do 2 wp_lam.
+      wp_bind (hash _ _).
+      iApply (wp_wand).
+      iApply (hash_spec _ _ _ HKey).
+      iIntros (h) "%".
+      iSimplifyEq.
+      wp_proj.
+      wp_load.
+      iApply (wp_wand).
+      iApply (modulo_spec).
+      iIntros (f) "%".
+      iSimplifyEq.
+      rewrite Z2Nat_inj_mod.
+      by iApply ("HΦ").
     Qed.      
+     (* iIntros "!# [% [% [% HTable]]]".
+      iDestruct "HTable" as (lSize lCap arr) "[% [Harr [HlData [HlSize HlCap]]]]".
+      do 2 wp_lam.
+      wp_bind (hash _ _).
+      iApply (wp_wand).
+      iApply (hash_spec K k' k HKey).
+      iIntros (h) "Hh".
+      iSimplifyEq.
+      wp_proj.
+      wp_load.
+      iApply (wp_wand).
+      iApply (modulo_spec).
+      iIntros (f) "Hf".
+      iSplit. done.
+      iSplit. done.
+      iSplit. done.
+      iSplit. done.
+      iExists lSize, lCap, arr.
+      by iFrame.
+    Qed.*)
+
+(* Uncommented for now as loops are hard to handle.
+
+    Lemma resize_loop_spec M M' data data' old new lArr lSize lCap i : 
+      content M data ->
+      content M' data' ->
+      (forall k, M' !! k = if decide (Hash K k mod length data' < i)
+                           then M !! k
+                           else None) ->
+      exists data'',
+        content M data'' /\
+        {{{lArr ↦ new ∗ lCap ↦ #(length data') ∗ array new (map bucket data')∗ array old (map bucket data) }}}
+          resize_loop #(length data) old (#lArr, #lSize, #lCap) #i
+          {{{ RET #(); lArr ↦ new ∗ lCap ↦ #(length data'') ∗ array new (map bucket data'')∗ array old (map bucket data)}}}.
+    Proof.
+      intros Hdata.
+      iLöb as "IH" forall (i).
+      Hdata' HM'.
+      eexists.
+      split; last first.
+      iIntros (Φ) "[HlArr [HlCap [Hnew Hold]]] HΦ".
+      iRevert (M' data') "Hnew HΦ".
       
+      
+    Lemma resize_spec t M :
+      {{{Table M t}}} resize t {{{ RET #(); Table M t }}}.
+    Proof.
+      iIntros (Φ) "HTable HΦ".
+      iDestruct "HTable" as (lData data) "[% [% [% HTable]]]".
+      iDestruct "HTable" as (lSize lCap arr) "[% [Harr [HlData [HlSize HlCap]]]]".
+      iSimplifyEq.
+      wp_lam.
+      do 2 wp_proj.
+      wp_load.
+      wp_lam.
+      wp_proj.
+      wp_load.
+      wp_lam.
+      do 2 wp_proj.
+      wp_op.
+      wp_bind (make_array _).
+      iApply (wp_wand).
+      rewrite -Nat2Z.inj_add.
+      iApply (make_array_spec (length data + length data) NONEV).
+      iIntros (newArr) "HnewArr".
+      wp_store.
+      wp_proj.
+      wp_op.
+      wp_store.
+      iApply (wp_wand with "[Harr HnewArr]").
+      
+      rewrite -Nat2Z.inj_0.
+      generalize 0 as i.
+      iIntros (i).
+      iLöb as "IH" forall (i).
+      *)
+
+    Lemma list_fmap_insert `(f: A -> B) (l : list A) i x :
+      f <$> (<[i := x]> l) = <[i := f x]> (f <$> l).
+    Proof.
+      revert i.
+      induction l as [| y l' IH] ; [done|].
+      intros [|i] ; [done|].
+      csimpl.
+      by rewrite IH.
+    Qed.
+      
+    Lemma insert_impl_spec (t k x : val) M k' :
+      as_key K k = Some k' -> {{{Table M t}}} insert_impl t k x {{{RET #(); Table (<[k' := x]>M) t}}}.
+    Proof.
+      intro HKey.
+      iIntros (Φ) "HTable HΦ".
+      iDestruct "HTable" as (lArr data) "[% [% [% HTable]]]".
+      iDestruct "HTable" as (lSize lCap arr) "[% [Harr [HlArr [HlSize HlCap]]]]".
+      iSimplifyEq.
+      do 3 wp_lam.
+      wp_bind (index _ _).
+      Check index_spec.
+      wp_apply (index_spec lArr lSize lCap k M k' (fmap bucket data) HKey with "[HlCap]").
+      by rewrite map_length.
+      iIntros "HlCap".
+      wp_lam.
+      do 2 wp_proj.
+      wp_load.
+      do 2 wp_proj.
+      wp_load.
+      assert (Hash K k' `mod` length data < length data) as HLen.
+      { apply Nat.mod_upper_bound. unfold gt in *. Nat.order. }
+      assert (exists l, data !! (Hash K k' `mod` length data) = Some l) as HSome.
+      by apply lookup_lt_is_Some_2.
+      destruct HSome as [l HSome].
+      Check list_lookup_fmap.
+      pose proof (list_lookup_fmap bucket data (Hash K k' `mod` length data)) as HBucket.
+      rewrite HSome in HBucket.
+      simpl in HBucket.
+      iPoseProof  (array_load_spec _ _ _ _ HBucket) as "arrLoadSpec".
+      iDestruct ("arrLoadSpec" with "Harr") as "H".
+      wp_bind (array_load _).
+      rewrite fmap_length.
+      iApply (wp_wand with "H") .
+      iIntros (v) "[% Harr]".
+      iSimplifyEq.
+      assert (Hash K k' `mod` length (bucket <$> data) < length (bucket <$> data)) as HLenFmap.
+      by rewrite fmap_length.
+      iPoseProof  (array_store_spec _ _ (SOMEV (k, x, bucket l)) _ HLenFmap) as "arrStoreSpec".
+      iDestruct ("arrStoreSpec" with "Harr") as "H".
+      wp_bind (array_store _).
+      rewrite fmap_length.
+      iApply (wp_wand with "H").
+      iIntros (v) "Harr".
+      wp_lam.
+      do 2 wp_proj.
+      wp_load.
+      wp_op.
+      wp_lam.
+      do 2 wp_proj.
+      wp_store.
+      wp_proj.
+      wp_load.
+      wp_lam.
+      iApply "HΦ".
+      iExists lArr,  (insertData data k' (k, x)). 
+      iSplit.
+      iPureIntro.
+      by rewrite insert_length.
+      iSplit.
+      iPureIntro.
+      by apply content_insert.
+      iSplit.
+      iPureIntro.
+      by apply no_garbage_insert.
+      iExists lSize, lCap, arr. 
+      iSplit ; [done|].
+      iSplitL "Harr".
+      unfold insertData.
+      unfold lookupData.
+      rewrite list_fmap_insert.
+      rewrite HSome.
+      simpl.
+      iFrame.
+      iFrame.
+      iSplitL "HlSize".
+      unfold insertData.
       
       
       
